Stacking*: Allow some of the frame data to lie above the stack data. ia32/Stacklayout: take advantage of this to put the return address   at the top of the Mach stack frame ia32/Conventions1: inefficient numbering of callee-save regs ia32/PrintAsm: adapted to new return address placement.
git-svn-id: https://yquem.inria.fr/compcert/svn/compcert/branches/unsigned-offsets@1625 fca1b0fc-160b-0410-b1d3-a4f43f01ea2e

ia32/PrintAsm.ml
@@ -167,9 +167,10 @@ let int32_align n a =
 
 let sp_adjustment sz =
   let sz = camlint_of_coqint sz in
-(* Enforce stack alignment, noting that 4 bytes are already allocated
-   by the call *)
-  let sz = Int32.sub (int32_align (Int32.add sz 4l) stack_alignment) 4l in
+  (* Preserve proper alignment of the stack *)
+  let sz = int32_align sz stack_alignment in
+  (* The top 4 bytes have already been allocated by the "call" instruction. *)
+  let sz = Int32.sub sz 4l in
   assert (sz >= 0l);
   sz
 
